isabelle/Chapter16_4_Abbreviations.thy
@@ -1,0 +1,99 @@
+theory Chapter16_4_Abbreviations
+imports Chapter16_3_Evaluation
+begin
+
+abbreviation Nat :: type
+where "Nat == Rec (Sum Unit (Tyvar 0))"
+
+lemma "is_valid_type {} Nat" by simp
+lemma "free_type_vars Nat = {}" by simp
+lemma "type_sub_from n Nat = Nat" by simp
+lemma "type_incr_from n Nat = Nat" by simp
+lemma "type_subst Nat t x = Nat" by simp
+
+abbreviation Zero :: expr
+where "Zero == Fold (Sum Unit (Tyvar 0)) (InL Unit Nat Triv)"
+
+lemma "free_vars Zero = {}" by simp
+lemma "incr_from n Zero = Zero" by simp
+lemma "sub_from n Zero = Zero" by simp
+lemma "subst Zero e x = Zero" by simp
+lemma "typecheck env Zero Nat" by (simp add: safe_type_subst_def)
+lemma "is_val Zero" by simp
+
+abbreviation Succ :: "expr => expr"
+where "Succ e == Fold (Sum Unit (Tyvar 0)) (InR Unit Nat e)"
+
+lemma "free_vars (Succ e) = free_vars e" by simp
+lemma "incr_from n (Succ e) = Succ (incr_from n e)" by simp
+lemma "sub_from n (Succ e) = Succ (sub_from n e)" by simp
+lemma "subst (Succ n) e x = Succ (subst n e x)" by simp
+lemma "typecheck env n Nat ==> typecheck env (Succ n) Nat" by (simp add: safe_type_subst_def)
+
+lemma "is_val (Succ n) = is_val n" by simp
+lemma "eval n n' ==> eval (Succ n) (Succ n')" by simp
+
+abbreviation IsZ :: "expr => expr => expr => expr"
+where "IsZ e0 e1 et == Case (Unfold et) (incr_from 0 e0) e1"
+
+lemma "free_vars (IsZ e0 e1 et) = free_vars e0 Un free_vars et Un redr_set (free_vars e1)" by auto
+lemma "incr_from n (IsZ e0 e1 et) = IsZ (incr_from n e0) (incr_from (Suc n) e1) (incr_from n et)" by simp
+lemma "sub_from n (IsZ e0 e1 et) = IsZ (sub_from n e0) (sub_from (Suc n) e1) (sub_from n et)"  by simp
+lemma "subst (IsZ e0 e1 et) e x = IsZ (subst e0 e x) (subst e1 (incr_from 0 e) (Suc x)) (subst et e x)" by simp
+lemma "typecheck env e Nat ==> typecheck env e0 t ==> typecheck (extend_at env 0 Nat) e1 t ==> typecheck env (IsZ e0 e1 e) t" 
+proof -
+  assume "typecheck env e Nat" 
+     and "typecheck env e0 t" 
+     and "typecheck (extend_at env 0 Nat) e1 t"
+  moreover hence "typecheck env (Unfold e) (safe_type_subst (Sum Unit (Tyvar 0)) (Rec (Sum Unit (Tyvar 0))))" by simp
+  ultimately show "typecheck env (Case (Unfold e) (incr_from 0 e0) e1) t" by (simp add: safe_type_subst_def)
+qed
+lemma "is_val (IsZ e0 e1 e2) = False" by simp
+lemma "eval e e' ==> eval (IsZ e0 e1 e) (IsZ e0 e1 e')" by simp
+lemma "EX e'. eval (IsZ e0 e1 Zero) e' & eval e' e0" 
+proof -
+  have "eval (Case (InL Unit Nat Triv) (incr_from 0 e0) e1) (safe_subst (incr_from 0 e0) Triv)" by (metis ecs2 is_val.simps(5))
+  hence "eval (Case (InL Unit Nat Triv) (incr_from 0 e0) e1) e0" by simp
+  moreover have "eval (Case (Unfold (Fold (Sum Unit (Tyvar 0)) (InL Unit Nat Triv))) (incr_from 0 e0) e1) (Case (InL Unit Nat Triv) (incr_from 0 e0) e1)" by simp
+  ultimately have "EX e'. eval (Case (Unfold (Fold (Sum Unit (Tyvar 0)) (InL Unit Nat Triv))) (incr_from 0 e0) e1) e' & eval e' e0" by fast
+  thus "EX e'. eval (IsZ e0 e1 Zero) e' & eval e' e0" by simp
+qed
+lemma "is_val e ==> EX e'. eval (IsZ e0 e1 (Succ e)) e' & eval e' (safe_subst e1 e)" 
+proof -
+  assume X: "is_val e"
+  hence "eval (Case (Unfold (Fold (Sum Unit (Tyvar 0)) (InR Unit Nat e))) (incr_from 0 e0) e1) (Case (InR Unit Nat e) (incr_from 0 e0) e1)" by simp
+  moreover with X have "eval (Case (InR Unit Nat e) (incr_from 0 e0) e1) (safe_subst e1 e)" by simp
+  ultimately show "EX e'. eval (IsZ e0 e1 (Succ e)) e' & eval e' (safe_subst e1 e)" by auto
+qed
+
+lemma canonical_nat: "typecheck env e Nat ==> is_val e ==> e = Zero | (EX v. typecheck env v Nat & is_val v & e = Succ v)"
+proof (induction env e Nat rule: typecheck.induct) 
+case tvar
+  thus ?case by simp
+next case tapp
+  thus ?case by simp
+next case tprl
+  thus ?case by simp
+next case tprr
+  thus ?case by simp
+next case tfix
+  thus ?case by simp
+next case tabt
+  thus ?case by simp
+next case tcse
+  thus ?case by simp
+next case (tfld env e)
+  from tfld have X: "typecheck env e (Sum Unit Nat)" by (simp add: safe_type_subst_def)
+  from tfld have "Sum Unit Nat = Nat \<Longrightarrow> e = Zero \<or> (\<exists>v. typecheck env v Nat \<and> is_val v \<and> e = Succ v)" by (simp add: safe_type_subst_def)
+  from tfld have Y: "is_val e" by simp
+
+  from X Y have "(EX e'. e = InL Unit Nat e' & is_val e' & typecheck env e' Unit) 
+               | (EX e'. e = InR Unit Nat e' & is_val e' & typecheck env e' Nat)" by (simp add: canonical_sum)
+
+  have "e = InL Unit Nat Triv | (EX v. typecheck env v Nat & is_val v & e = InR Unit Nat v)" by simp sorry
+  thus ?case by simp
+next case tufd
+  thus ?case by simp
+qed
+
+end
